Let $Y=n-X$ and let $\nu=\E{Y}$.
By linearity of expectation, $\nu=n-\E{X}=n-\mu$.
Since $r>\nu$, we can use Theorem C.8 to obtain
\begin{align*}
    \Pr{\mu-X\ge r} &= \Pr{n-\nu-X\ge r} \\
    &= \Pr{Y-\nu\ge r} \\
    &\le \left(\frac{\nu e}{r}\right)^r \\
    &= \left(\frac{(n-\mu)e}{r}\right)^r.
\end{align*}

Similarly, in the second part, if we let $Y=n-X$, then $\E{Y}=n-\E{X}=n-np=nq$.
Since $r>nq$, we use Corollary C.9 to get
\begin{align*}
    \Pr{np-X\ge r} &= \Pr{n-nq-X\ge r} \\
    &= \Pr{Y-nq\ge r} \\
    &\le \left(\frac{nqe}{r}\right)^r.
\end{align*}
