The right-hand side of inequality (C.51) can be expressed as the function $f(\alpha)=\exp(\mu e^\alpha-\alpha r)$, where $\alpha>0$ and $r>\mu>0$.
We examine its derivatives:
\begin{align*}
    f'(\alpha) &= (\mu e^\alpha-r)\exp(\mu e^\alpha-\alpha r), \\
    f''(\alpha) &= \left(\mu e^\alpha+(\mu e^\alpha-r)^2\right)\exp(\mu e^\alpha-\alpha r).
\end{align*}
$f'(\alpha)=0$ for $\alpha=\ln(r/\mu)$, and $f''(\alpha)>0$ for all $\alpha>0$.
Therefore, $f(\alpha)$ is minimized at $\alpha=\ln(r/\mu)$.
