We prove the three properties of the loop invariant:
\begin{description}
    \item[Initialization:] Prior to the first iteration, $i=n$, so
    \begin{align*}
        p &= \sum_{k=0}^{n-(i+1)}A[k+i+1]\cdot x^k \\
        &= \sum_{k=0}^{-1}A[k+n+1]\cdot x^k \\
        &= 0,
    \end{align*}
    that matches the initial value of $p$.
    \item[Maintenance:] During each iteration $p$ gets the value of $A[i]+x\cdot p$.
    Assuming that the invariant holds before the current iteration, we have
    \begin{align*}
        p &= A[i]+\sum_{k=0}^{n-(i+1)}A[k+i+1]\cdot x^{k+1} \\
        &= A[i]\cdot x^0+\sum_{k=1}^{n-i}A[k+i]\cdot x^k \\
        &= \sum_{k=0}^{n-i}A[k+i]\cdot x^k.
    \end{align*}
    After decrementing $i$ for the next iteration, the invariant is preserved.
    \item[Termination:] The loop terminates, since it performs exactly $n+1$ iterations.
    At termination, $i=-1$, so
    \begin{align*}
        p &= \sum_{k=0}^{n-(i+1)}A[k+i+1]\cdot x^k \\
        &= \sum_{k=0}^nA[k]\cdot x^k.
    \end{align*}
    Therefore, the algorithm correctly evaluates the polynomial $P(x)$ for a given $x$.
\end{description}
